TypModels.v
@@ -1,0 +1,215 @@
+Require Import Models.
+
+Module Type Judge.
+    Parameter sub : Type.
+  Module T.
+    Parameter term : Type.
+    Parameter eq_term : term -> term -> Prop.
+    Parameter prop kind : term.
+    Parameter Ref : nat -> term.
+    Parameter App Abs Prod : term -> term -> term.
+
+    Parameter eq_sub : sub -> sub -> Prop.
+    Parameter sub_id : sub.
+    Parameter sub_comp : sub -> sub -> sub.
+    Parameter sub_lift : nat -> sub -> sub.
+    Parameter sub_shift : nat -> sub.
+    Parameter sub_cons : term -> sub -> sub.
+
+    Parameter Sub : term -> sub -> term.
+
+    Parameter lift : nat -> term -> term.
+    Parameter lift1 : nat -> term -> term.
+    Parameter subst : term -> term -> term.
+  End T.
+  Import T.
+
+  Definition env : Type := list term.
+
+  Module J.
+    Parameter typ eq_typ sub_typ : env -> term -> term -> Prop.
+    Parameter typ_sub : env -> sub -> env -> Prop.
+  End J.
+  Import J.
+
+  Module R.
+    (** Equivalence and congruence rules *)
+    Parameter refl : forall e M, eq_typ e M M.
+    Parameter sym : forall e M M', eq_typ e M M' -> eq_typ e M' M. 
+    Parameter trans : forall e M M' M'',
+      eq_typ e M M' -> eq_typ e M' M'' -> eq_typ e M M''.
+
+    Parameter eq_typ_app : forall e M M' N N',
+      eq_typ e M M' ->
+      eq_typ e N N' ->
+      eq_typ e (App M N) (App M' N').
+
+    Parameter eq_typ_abs : forall e T T' M M',
+      eq_typ e T T' ->
+      eq_typ (T::e) M M' ->
+      eq_typ e (Abs T M) (Abs T' M').
+
+    Parameter eq_typ_prod : forall e T T' U U',
+      eq_typ e T T' ->
+      eq_typ (T::e) U U' ->
+      eq_typ e (Prod T U) (Prod T' U').
+
+    Parameter eq_typ_beta : forall e T M M' N N',
+      eq_typ (T::e) M M' ->
+      eq_typ e N N' ->
+      typ e N T -> (* Typed reduction! *)
+      T <> kind ->
+      eq_typ e (App (Abs T M) N) (subst N' M').
+
+
+    (** Typing rules *)
+    Parameter typ_prop : forall e, typ e prop kind.
+
+    Parameter typ_var : forall e n T,
+      nth_error e n = value T ->
+      typ e (Ref n) (lift (S n) T).
+
+    Parameter typ_app : forall e u v V Ur,
+      typ e v V ->
+      typ e u (Prod V Ur) ->
+      V <> kind ->
+      typ e (App u v) (subst v Ur).
+
+    Parameter typ_abs : forall e T M U,
+      typ (T :: e) M U ->
+      U <> kind ->
+      typ e (Abs T M) (Prod T U).
+
+    Parameter typ_prod : forall e T U s2,
+      s2 = kind \/ s2 = prop ->
+      typ (T :: e) U s2 ->
+      typ e (Prod T U) s2.
+
+    Parameter typ_conv : forall e M T T',
+      typ e M T ->
+      eq_typ e T T' ->
+      T <> kind ->
+      typ e M T'.
+
+
+    (** Subtyping *)
+    Parameter sub_refl : forall e M M',
+      eq_typ e M M' -> sub_typ e M M'.
+
+    Parameter sub_trans : forall e M1 M2 M3,
+      sub_typ e M1 M2 -> sub_typ e M2 M3 -> sub_typ e M1 M3.
+
+    Parameter typ_subsumption : forall e M T T',
+      typ e M T ->
+      sub_typ e T T' ->
+      T <> kind ->
+      typ e M T'.
+
+
+    (** Substitution *)
+    Parameter typ_sub_comp : forall e f g s1 s2,
+      typ_sub e s1 f ->
+      typ_sub f s2 g ->
+      typ_sub e (sub_comp s2 s1) g.
+
+    Parameter typ_Sub : forall e f s m u,
+      typ f m u ->
+      typ_sub e s f ->
+      typ e (Sub m s) (Sub u s).
+
+    Parameter typ_sub_shift1 : forall e ty,
+      typ_sub (ty::e) (sub_shift 1) e.
+
+    Parameter typ_sub_lams1 : forall e s f t,
+      typ_sub e s f ->
+      typ_sub (Sub t s :: e) (sub_lift 1 s) (t::f).
+
+    (** Admissible rules *)
+    (* TODO: weakening is an instance of typ_Sub *)
+    Parameter weakening : forall e M T A,
+      typ e M T ->
+      typ (A::e) (lift 1 M) (lift 1 T).
+
+  End R.
+
+End Judge.
+
+Module Type ECC_Rules (M:Judge).
+  Import M M.T M.J.
+
+  Parameter type : nat -> term.
+
+  Parameter typ_Prop : forall e, typ e prop (type 0).
+
+  Parameter typ_Type : forall e n, typ e (type n) (type (S n)).
+  Parameter cumul_Type : forall e n, sub_typ e (type n) (type (S n)).
+  Parameter cumul_Prop : forall e, sub_typ e prop (type 0).
+
+  Parameter typ_prod2 : forall e n T U,
+    typ e T (type n) ->
+    typ (T :: e) U (type n) ->
+    typ e (Prod T U) (type n).
+
+  Parameter sub_typ_covariant : forall e U1 U2 V1 V2,
+    U1 <> kind ->
+    eq_typ e U1 U2 ->
+    sub_typ (U1::e) V1 V2 ->
+    sub_typ e (Prod U1 V1) (Prod U2 V2).
+
+End ECC_Rules.
+
+Module Type Nat_Rules (M:Judge).
+  Import M M.T M.J.
+
+  Parameter Nat Zero Succ : term.
+  Parameter NatRec : term -> term -> term -> term.
+
+  Parameter typ_N : forall e, typ e Nat kind.
+  Parameter typ_0 : forall e, typ e Zero Nat.
+  Parameter typ_S : forall e, typ e Succ (Prod Nat (lift 1 Nat)).
+  Parameter typ_Nrect : forall e n f g P,
+    typ e n Nat ->
+    typ e f (App P Zero) ->
+    typ e g (Prod Nat (Prod (App (lift 1 P) (Ref 0))
+               (App (lift 2 P) (App Succ (Ref 1))))) ->
+    typ e (NatRec f g n) (App P n).
+
+  Parameter eq_typ_NatRec : forall e f f' g g' n n',
+    eq_typ e f f' ->
+    eq_typ e g g' ->
+    eq_typ e n n' ->
+    eq_typ e (NatRec f g n) (NatRec f' g' n').
+
+  Parameter NatRec_eq_0 : forall e f g,
+    eq_typ e (NatRec f g Zero) f.
+
+  Parameter NatRec_eq_S : forall e f g n,
+    typ e n Nat ->
+    eq_typ e (NatRec f g (App Succ n)) (App (App g n) (NatRec f g n)).
+
+End Nat_Rules.
+
+Module Type W_Rules (M:Judge).
+  Import M M.T M.J.
+
+  (*Parameter Ordt : set -> term. *)
+  Parameter OSucc : term -> term.
+  Parameter OSucct : term -> term.
+
+  Parameter WI : term -> term -> term -> term.
+  Parameter Wc : term -> term -> term -> term -> term.
+  Parameter Wcase : term -> term -> term -> term -> term.
+  Parameter WFix : term -> term -> term -> term -> term.
+
+End W_Rules.
+
+Module Type Variance (M:Judge).
+  Import M M.T M.J.
+
+  Parameter fenv_ : Type.
+  Parameter tenv : fenv_ -> env.
+  Parameter push_var : fenv_ -> term -> fenv_.
+  Parameter push_ord : fenv_ -> term -> fenv_.
+  Parameter push_fun : fenv_ -> term -> term -> fenv_.
+  Parameter var_equals : fenv_ -> term -> Prop.
+End Variance.
